# MIT License
#
# Copyright (c) 2021 Markus Schröder, DFKI GmbH
#
# Permission is hereby granted, free of charge, to any person obtaining a copy
# of this software and associated documentation files (the "Software"), to deal
# in the Software without restriction, including without limitation the rights
# to use, copy, modify, merge, publish, distribute, sublicense, and/or sell
# copies of the Software, and to permit persons to whom the Software is
# furnished to do so, subject to the following conditions:
#
# The above copyright notice and this permission notice shall be included in all
# copies or substantial portions of the Software.
#
# THE SOFTWARE IS PROVIDED "AS IS", WITHOUT WARRANTY OF ANY KIND, EXPRESS OR
# IMPLIED, INCLUDING BUT NOT LIMITED TO THE WARRANTIES OF MERCHANTABILITY,
# FITNESS FOR A PARTICULAR PURPOSE AND NONINFRINGEMENT. IN NO EVENT SHALL THE
# AUTHORS OR COPYRIGHT HOLDERS BE LIABLE FOR ANY CLAIM, DAMAGES OR OTHER
# LIABILITY, WHETHER IN AN ACTION OF CONTRACT, TORT OR OTHERWISE, ARISING FROM,
# OUT OF OR IN CONNECTION WITH THE SOFTWARE OR THE USE OR OTHER DEALINGS IN THE
# SOFTWARE.

@prefix rdfs: <http://www.w3.org/2000/01/rdf-schema#> .
@prefix rdf: <http://www.w3.org/1999/02/22-rdf-syntax-ns#>.
@prefix xsd: <http://www.w3.org/2001/XMLSchema#>.
@prefix dc: <http://purl.org/dc/elements/1.1/> .
@prefix owl: <http://www.w3.org/2002/07/owl#> .
@prefix foaf: <http://xmlns.com/foaf/0.1/> .

@prefix : <http://localhost:8081/ontology> .
@prefix ex: <http://localhost:8081/ontology/> .

: a owl:Ontology ;
    dc:creator "Markus Schröder" ;
    dc:date "2021-03-04"^^xsd:date ;
    dc:title "Guideline Ontology" ;
    dc:description "This ontology contains the terminology to describe managed guideline documents." .

ex:Guideline a rdfs:Class ;
    rdfs:subClassOf foaf:Document ;
    rdfs:label "Guideline" ;
    rdfs:comment "A guideline is a document that contains statements used to determine a course of action. It aims to streamline particular processes according to a set routine or sound practice." .

ex:Attachment a rdfs:Class ;
    rdfs:subClassOf foaf:Document ;
    rdfs:label "Attachment" ;
    rdfs:comment "A document joined to a guideline which gives extra details." .

ex:Department a rdfs:Class ;
    rdfs:label "Department" ;
    rdfs:comment "A part of an organization that deals with a particular area of work." .

ex:Kind a rdfs:Class ;
    rdfs:label "Kind" ;
    rdfs:comment "A group with similar characteristics, or a particular type of guidelines." .

ex:State a rdfs:Class ;
    rdfs:label "State" ;
    rdfs:comment "A condition of a document that exists at a particular time." .

ex:Category a rdfs:Class ;
    rdfs:label "Category" ;
    rdfs:comment "A group of guidelines having some features that are the same." .

ex:MailingList a rdfs:Class ;
    rdfs:label "Mailing List" ;
    rdfs:comment "A list of names and addresses kept by an organization so that it can notify changes in guidelines." .

ex:SecurityNeed a rdfs:Class ;
    rdfs:label "Security Need" ;
    rdfs:comment "A need for security by a guideline because of confidentiality reasons." .

ex:Procedure a rdfs:Class ;
    rdfs:label "Procedure" ;
    rdfs:comment "A set of actions that has to be done to manage a guideline." .

ex:Progress a rdfs:Class ;
    rdfs:label "Progress" ;
    rdfs:comment "A progress status for estimating development towards a completed procedure." .

ex:manages a rdf:Property ;
    rdfs:label "Manages" ;
    rdfs:comment "A procedure manages a certain guideline." ;
    rdfs:domain ex:Procedure ;
    rdfs:range ex:Guideline .

ex:hasProgress a rdf:Property ;
    rdfs:label "Progress" ;
    rdfs:comment "A procedure has reached a certain progress." ;
    rdfs:domain ex:Procedure ;
    rdfs:range ex:Progress .

ex:hasId a rdf:Property ;
    rdfs:label "ID" ;
    rdfs:comment "A unique identification string used to refer to a particular guideline." ;
    rdfs:domain ex:Guideline ;
    rdfs:range xsd:string .

ex:hasNumber a rdf:Property ;
    rdfs:label "Number" ;
    rdfs:comment "A unique identification number used to refer to a particular attachment." ;
    rdfs:domain ex:Attachment ;
    rdfs:range xsd:int .

ex:validFrom a rdf:Property ;
    rdfs:label "Valid From" ;
    rdfs:comment "The date when a document is in the condition of being officially true or legally acceptable." ;
    rdfs:domain ex:Guideline , ex:Attachment ;
    rdfs:range xsd:date ;
    rdfs:seeAlso ex:invalidFrom .

ex:plannedValidFrom a rdf:Property ;
    rdfs:label "Planned Valid From" ;
    rdfs:comment "The date when a document is planned to be officially true or legally acceptable." ;
    rdfs:domain ex:Guideline , ex:Attachment ;
    rdfs:range xsd:date ;
    rdfs:seeAlso ex:validFrom .

ex:invalidFrom a rdf:Property ;
    rdfs:label "Invalid From" ;
    rdfs:comment "The date when a document is in the condition of not being legally or officially acceptable." ;
    rdfs:domain ex:Guideline , ex:Attachment ;
    rdfs:range xsd:date ;
    rdfs:seeAlso ex:validFrom .

ex:lastModifiedDate a rdf:Property ;
    rdfs:label "Last Modified Date" ;
    rdfs:comment "The date when a document was last edited or changed." ;
    rdfs:domain ex:Guideline , ex:Attachment ;
    rdfs:range xsd:date .

ex:isRecent a rdf:Property ;
    rdfs:label "Recent" ;
    rdfs:comment "A boolean value if the guideline was introduced and not managed yet." ;
    rdfs:domain ex:Guideline ;
    rdfs:range xsd:boolean .

ex:hasCategory a rdf:Property ;
    rdfs:label "Category" ;
    rdfs:comment "A guideline is associated with a certain category." ;
    rdfs:domain ex:Guideline ;
    rdfs:range ex:Category .

ex:hasNote a rdf:Property ;
    rdfs:label "Note" ;
    rdfs:comment "A short note about a document." ;
    rdfs:domain ex:Guideline , ex:Attachment ;
    rdfs:range xsd:string .

ex:hasAttachment a rdf:Property ;
    rdfs:label "Attachment" ;
    rdfs:comment "A guideline has an attachment." ;
    rdfs:domain ex:Guideline ;
    rdfs:range ex:Attachment .

ex:hasAbbreviation a rdf:Property ;
    rdfs:label "Abbreviation" ;
    rdfs:comment "A short form of a title or name of something (e.g. an acronym)." ;
    rdfs:domain rdf:Resource ;
    rdfs:range xsd:string .

ex:hasState a rdf:Property ;
    rdfs:label "State" ;
    rdfs:comment "A state in which the document currently is." ;
    rdfs:domain ex:Guideline , ex:Attachment ;
    rdfs:range ex:State .

ex:hasSecurityNeed a rdf:Property ;
    rdfs:label "Security Need" ;
    rdfs:comment "The security need the guideline currently has." ;
    rdfs:domain ex:Guideline ;
    rdfs:range ex:SecurityNeed .

ex:hasDepartment a rdf:Property ;
    rdfs:label "Department" ;
    rdfs:comment "A guideline applies to a certain department." ;
    rdfs:domain ex:Guideline ;
    rdfs:range ex:Department .

ex:worksAt a rdf:Property ;
    rdfs:label "Works At" ;
    rdfs:comment "A person works at a certain department or in a certain group." ;
    rdfs:domain foaf:Person ;
    rdfs:range xsd:string .

ex:inMailingList a rdf:Property ;
    rdfs:label "Mailing List" ;
    rdfs:comment "A guideline is associated with a mailing list." ;
    rdfs:domain ex:Guideline ;
    rdfs:range ex:MailingList .

ex:hasTitle a rdf:Property ;
    rdfs:subPropertyOf dc:title ;
    rdfs:label "Title" ;
    rdfs:comment "A headline of a document." ;
    rdfs:domain ex:Guideline , ex:Attachment ;
    rdfs:range xsd:string .

ex:hasKind a rdf:Property ;
    rdfs:label "Kind" ;
    rdfs:comment "A guildline is from a specific kind (type, category)." ;
    rdfs:domain ex:Guideline ;
    rdfs:range ex:Kind .

ex:hasEditorResponsible a rdf:Property ;
    rdfs:subPropertyOf ex:hasEditor ;
    rdfs:label "Responsible" ;
    rdfs:comment "A guideline has a responsible editor who makes important decisions for the guideline." ;
    rdfs:domain ex:Guideline , ex:Attachment ;
    rdfs:range foaf:Person .

ex:hasEditor a rdf:Property ;
    rdfs:label "Editor" ;
    rdfs:comment "A document has an editor who changes the content of a document." ;
    rdfs:domain ex:Guideline , ex:Attachment ;
    rdfs:range foaf:Person .

ex:wasFormerEditor a rdf:Property ;
    rdfs:label "Former Editor" ;
    rdfs:comment "A document had an editor who changed the content of a document." ;
    rdfs:domain ex:Guideline , ex:Attachment ;
    rdfs:range foaf:Person .

ex:hasReviewer a rdf:Property ;
    rdfs:label "Reviewer" ;
    rdfs:comment "A guideline has an reviewer who checks the content of a guideline." ;
    rdfs:domain ex:Guideline ;
    rdfs:range foaf:Person .

